<?xml version="1.0"?>
<rdf:RDF xmlns="https://spec.industrialontologies.org/ontology/qualities/"
     xml:base="https://spec.industrialontologies.org/ontology/qualities/"
     xmlns:dc="http://purl.org/dc/elements/1.1/"
     xmlns:obo="http://purl.obolibrary.org/obo/"
     xmlns:owl="http://www.w3.org/2002/07/owl#"
     xmlns:rdf="http://www.w3.org/1999/02/22-rdf-syntax-ns#"
     xmlns:xml="http://www.w3.org/XML/1998/namespace"
     xmlns:xsd="http://www.w3.org/2001/XMLSchema#"
     xmlns:prov="http://www.w3.org/ns/prov#"
     xmlns:rdfs="http://www.w3.org/2000/01/rdf-schema#"
     xmlns:skos="http://www.w3.org/2004/02/skos/core#"
     xmlns:iof-av="https://spec.industrialontologies.org/ontology/core/meta/AnnotationVocabulary/"
     xmlns:dcterms="http://purl.org/dc/terms/"
     xmlns:iof-core="https://spec.industrialontologies.org/ontology/core/Core/"
     xmlns:AnnotationVocabulary="https://www.omg.org/spec/Commons/AnnotationVocabulary/">
    <owl:Ontology rdf:about="https://spec.industrialontologies.org/ontology/qualities/Qualities-MeasurementPerformance/">
        <owl:imports rdf:resource="https://spec.industrialontologies.org/ontology/qualities/Qualities/"/>
        <dcterms:abstract xml:lang="en-us">This Submodule, Measurement Performance Qualities, of the IOF Qualities Ontology aims to represent the generic constructs (including classes and properties) related bfo qualities covering Measurement Performance.</dcterms:abstract>
        <dcterms:contributor xml:lang="en-us">Thomas Hanke, Fraunhofer IWM</dcterms:contributor>
        <dcterms:creator xml:lang="en-us">IOF Materials Working Group</dcterms:creator>
        <dcterms:license rdf:datatype="http://www.w3.org/2001/XMLSchema#anyURI">http://opensource.org/licenses/MIT</dcterms:license>
        <dcterms:publisher>Industrial Ontology Foundry</dcterms:publisher>
        <dcterms:title xml:lang="en-us">Industrial Ontology Foundry (IOF) Process Qualities Ontology</dcterms:title>
        <rdfs:label xml:lang="en-us">Measurement Performance Qualities Ontology</rdfs:label>
        <iof-av:copyright>Industrial Ontology Foundry (IOF)</iof-av:copyright>
        <iof-av:maturity rdf:resource="https://spec.industrialontologies.org/ontology/core/meta/AnnotationVocabulary/Provisional"/>
    </owl:Ontology>


    <!-- 
    ///////////////////////////////////////////////////////////////////////////////////////
    //
    // Annotation properties
    //
    ///////////////////////////////////////////////////////////////////////////////////////
     -->

    


    <!-- http://purl.obolibrary.org/obo/IAO_0000114 -->

    <owl:AnnotationProperty rdf:about="http://purl.obolibrary.org/obo/IAO_0000114">
        <rdfs:label xml:lang="en">Has Curation Status</rdfs:label>
    </owl:AnnotationProperty>
    


    <!-- http://purl.obolibrary.org/obo/IAO_0000116 -->

    <owl:AnnotationProperty rdf:about="http://purl.obolibrary.org/obo/IAO_0000116">
        <rdfs:label xml:lang="en">Editor Note</rdfs:label>
    </owl:AnnotationProperty>
    


    <!-- http://purl.obolibrary.org/obo/IAO_0000117 -->

    <owl:AnnotationProperty rdf:about="http://purl.obolibrary.org/obo/IAO_0000117">
        <rdfs:label xml:lang="en">Term Editor</rdfs:label>
    </owl:AnnotationProperty>
    


    <!-- http://purl.obolibrary.org/obo/IAO_0000119 -->

    <owl:AnnotationProperty rdf:about="http://purl.obolibrary.org/obo/IAO_0000119">
        <rdfs:label xml:lang="en">Definition Source</rdfs:label>
    </owl:AnnotationProperty>
    


    <!-- http://purl.obolibrary.org/obo/IAO_0000412 -->

    <owl:AnnotationProperty rdf:about="http://purl.obolibrary.org/obo/IAO_0000412">
        <rdfs:label xml:lang="en">Imported From</rdfs:label>
    </owl:AnnotationProperty>
    


    <!-- http://purl.org/dc/terms/bibliographicCitation -->

    <owl:AnnotationProperty rdf:about="http://purl.org/dc/terms/bibliographicCitation"/>
    


    <!-- http://purl.org/dc/terms/created -->

    <owl:AnnotationProperty rdf:about="http://purl.org/dc/terms/created"/>
    


    <!-- http://purl.org/dc/terms/title -->

    <owl:AnnotationProperty rdf:about="http://purl.org/dc/terms/title"/>
    


    <!-- http://www.w3.org/ns/prov#editorialNote -->

    <owl:AnnotationProperty rdf:about="http://www.w3.org/ns/prov#editorialNote"/>
    


    <!-- 
    ///////////////////////////////////////////////////////////////////////////////////////
    //
    // Classes
    //
    ///////////////////////////////////////////////////////////////////////////////////////
     -->

    


    <!-- https://spec.industrialontologies.org/ontology/qualities/Qualities-MeasurementPerformance/CalibrationRange -->

    <owl:Class rdf:about="https://spec.industrialontologies.org/ontology/qualities/Qualities-MeasurementPerformance/CalibrationRange">
        <rdfs:subClassOf rdf:resource="https://spec.industrialontologies.org/ontology/qualities/Qualities-Physical/DynamicRange"/>
        <obo:IAO_0000114 rdf:resource="http://purl.obolibrary.org/obo/IAO_0000428"/>
        <rdfs:isDefinedBy rdf:resource="https://w3id.org/pmd/co"/>
        <rdfs:label xml:lang="en">Calibration Range</rdfs:label>
        <rdfs:label xml:lang="de">Kalibrierbereich</rdfs:label>
        <skos:definition xml:lang="de">Diese Eigenschaft beschreibt den Bereich zwischen den Grenzen, innerhalb derer eine Größe gemessen, empfangen oder übertragen wird (typischerweise von einem Prozessknoten, z. B. einer Maschine), ausgedrückt durch die Angabe des unteren und oberen Bereichswertes.</skos:definition>
        <skos:definition xml:lang="en">This property describes the region between the limits within which a quantity is measured, received or transmitted (typically by a process node, e.g. a machine), expressed by stating the lower and upper range values.</skos:definition>
    </owl:Class>
    


    <!-- https://spec.industrialontologies.org/ontology/qualities/Qualities-MeasurementPerformance/DataAcquisitionRate -->

    <owl:Class rdf:about="https://spec.industrialontologies.org/ontology/qualities/Qualities-MeasurementPerformance/DataAcquisitionRate">
        <rdfs:subClassOf rdf:resource="https://spec.industrialontologies.org/ontology/core/Core/ProcessCharacteristic"/>
        <rdfs:isDefinedBy rdf:resource="https://w3id.org/pmd/co"/>
        <rdfs:label xml:lang="en">Data Acquisition Rate</rdfs:label>
        <rdfs:label xml:lang="de">Datenerfassungsrate</rdfs:label>
        <skos:definition xml:lang="de">Diese Eigenschaft bezeichnet die Anzahl der Messungen / Abfragen pro Zeiteinheit bei einer betrachteten Messung einer Messgröße (Abtast-/Abfragerate bei der Datenerfassung).</skos:definition>
        <skos:definition xml:lang="en">This property denotes the number of measurements / queries per time period for a considered measurement of a measurement parameter (sampling / query rate during data acquisition).</skos:definition>
    </owl:Class>
    


    <!-- https://spec.industrialontologies.org/ontology/qualities/Qualities-MeasurementPerformance/MeasurementRelationalQuality -->

    <owl:Class rdf:about="https://spec.industrialontologies.org/ontology/qualities/Qualities-MeasurementPerformance/MeasurementRelationalQuality">
        <rdfs:subClassOf rdf:resource="http://purl.obolibrary.org/obo/BFO_0000145"/>
        <rdfs:label xml:lang="en">Measurement Relational Quality</rdfs:label>
    </owl:Class>
    


    <!-- https://spec.industrialontologies.org/ontology/qualities/Qualities-MeasurementPerformance/PerformanceQuality -->

    <owl:Class rdf:about="https://spec.industrialontologies.org/ontology/qualities/Qualities-MeasurementPerformance/PerformanceQuality">
        <rdfs:subClassOf rdf:resource="http://purl.obolibrary.org/obo/BFO_0000019"/>
        <rdfs:label xml:lang="de">Leistungsqualität</rdfs:label>
        <rdfs:label xml:lang="en">Performance Quality</rdfs:label>
        <obo:IAO_0000117>PERSON: Thomas Hanke</obo:IAO_0000117>
    </owl:Class>
    


    <!-- https://spec.industrialontologies.org/ontology/qualities/Qualities-MeasurementPerformance/Precision -->

    <owl:Class rdf:about="https://spec.industrialontologies.org/ontology/qualities/Qualities-MeasurementPerformance/Precision">
        <rdfs:subClassOf rdf:resource="https://spec.industrialontologies.org/ontology/qualities/Qualities-MeasurementPerformance/MeasurementRelationalQuality"/>
        <obo:IAO_0000114 rdf:resource="http://purl.obolibrary.org/obo/IAO_0000428"/>
        <obo:IAO_0000119 xml:lang="en">“Precision.” Merriam-Webster.com Dictionary, Merriam-Webster, https://www.merriam-webster.com/dictionary/precision. Accessed 13 Jan. 2023.</obo:IAO_0000119>
        <rdfs:isDefinedBy rdf:resource="https://w3id.org/pmd/co"/>
        <rdfs:label xml:lang="de">Genauigkeit</rdfs:label>
        <rdfs:label xml:lang="en">Precision</rdfs:label>
        <skos:definition xml:lang="de">Der Grad der Verfeinerung, mit dem eine Operation durchgeführt oder eine Messung angegeben wird.</skos:definition>
        <skos:definition xml:lang="en">The degree of refinement with which an operation is performed or a measurement stated.</skos:definition>
    </owl:Class>
    


    <!-- https://spec.industrialontologies.org/ontology/qualities/Qualities-MeasurementPerformance/WorkingRange -->

    <owl:Class rdf:about="https://spec.industrialontologies.org/ontology/qualities/Qualities-MeasurementPerformance/WorkingRange">
        <rdfs:subClassOf rdf:resource="https://spec.industrialontologies.org/ontology/qualities/Qualities-Physical/DynamicRange"/>
        <obo:IAO_0000114 rdf:resource="http://purl.obolibrary.org/obo/IAO_0000428"/>
        <rdfs:isDefinedBy rdf:resource="https://w3id.org/pmd/co"/>
        <rdfs:label xml:lang="de">Arbeitsbereich</rdfs:label>
        <rdfs:label xml:lang="en">Working Range</rdfs:label>
        <skos:definition xml:lang="de">Diese Eigenschaft beschreibt den Bereich zwischen den Grenzen, innerhalb derer ein Prozessknoten (z. B. eine Maschine) für ihren vorgesehenen Zweck verwendet werden kann, ausgedrückt durch die Angabe der in Rede stehenden unteren und oberen Bereichswerte.</skos:definition>
        <skos:definition xml:lang="en">This property describes the region between the limits within which a processing node (e.g., a machine) is capable of being used for its intended purpose, expressed by stating the lower and upper range values of interest.</skos:definition>
    </owl:Class>
    


    <!-- https://spec.industrialontologies.org/ontology/qualities/Qualities-Physical/DynamicRange -->

    <owl:Class rdf:about="https://spec.industrialontologies.org/ontology/qualities/Qualities-Physical/DynamicRange">
        <rdfs:subClassOf rdf:resource="https://spec.industrialontologies.org/ontology/qualities/Qualities-MeasurementPerformance/MeasurementRelationalQuality"/>
        <obo:IAO_0000119 xml:lang="en">https://en.wikipedia.org/wiki/Dynamic_range</obo:IAO_0000119>
        <rdfs:label xml:lang="en">Dynamic Range</rdfs:label>
        <rdfs:label xml:lang="de">Dynamikbereich</rdfs:label>
        <obo:IAO_0000117>PERSON: Thomas Hanke</obo:IAO_0000117>
        <iof-av:naturalLanguageDefinition xml:lang="en">Dynamic range (abbreviated DR, DNR or DYR) is the ratio between the largest and smallest values that a certain quantity can assume. It is often used in the context of signals, like sound and light. It is measured either as a ratio or as a base-10 (decibel) or base-2 (doublings, bits or stops) logarithmic value of the ratio between the largest and smallest signal values.</iof-av:naturalLanguageDefinition>
    </owl:Class>
</rdf:RDF>



<!-- Generated by the OWL API (version 4.5.26.2023-07-17T20:34:13Z) https://github.com/owlcs/owlapi -->

