<?xml version="1.0" encoding="UTF-8"?>
<!DOCTYPE rdf:RDF [
	<!ENTITY dcterms "http://purl.org/dc/terms/">
	<!ENTITY dtype "http://www.linkedmodel.org/schema/dtype#">
	<!ENTITY owl "http://www.w3.org/2002/07/owl#">
	<!ENTITY rdf "http://www.w3.org/1999/02/22-rdf-syntax-ns#">
	<!ENTITY rdfs "http://www.w3.org/2000/01/rdf-schema#">
	<!ENTITY vaem "http://www.linkedmodel.org/schema/vaem#">
	<!ENTITY voag "http://voag.linkedmodel.org/voag#">
	<!ENTITY xsd "http://www.w3.org/2001/XMLSchema#">
]>
<rdf:RDF xml:base="http://www.linkedmodel.org/schema/dtype"
	xmlns:dcterms="http://purl.org/dc/terms/"
	xmlns:dtype="http://www.linkedmodel.org/schema/dtype#"
	xmlns:owl="http://www.w3.org/2002/07/owl#"
	xmlns:rdf="http://www.w3.org/1999/02/22-rdf-syntax-ns#"
	xmlns:rdfs="http://www.w3.org/2000/01/rdf-schema#"
	xmlns:vaem="http://www.linkedmodel.org/schema/vaem#"
	xmlns:voag="http://voag.linkedmodel.org/voag#"
	xmlns:xsd="http://www.w3.org/2001/XMLSchema#">
	
	<owl:Ontology rdf:about="http://www.linkedmodel.org/schema/dtype">
		<rdfs:label>Datatype Ontology</rdfs:label>
		<dcterms:author>Ralph Hodgson</dcterms:author>
		<dcterms:subject>Datatype Schema</dcterms:subject>
		<dcterms:title>Datatype Ontology</dcterms:title>
		<vaem:hasGraphMetadata rdf:resource="&dtype;GMD_DTYPE"/>
		<owl:imports rdf:resource="http://www.linkedmodel.org/schema/vaem"/>
		<owl:versionIRI rdf:resource="http://www.linkedmodel.org/schema/dtype"/>
	</owl:Ontology>
	
	<owl:AnnotationProperty rdf:about="&dcterms;author">
		<rdfs:label>author</rdfs:label>
		<rdfs:isDefinedBy rdf:resource="http://purl.org/dc/terms/"/>
		<rdfs:range rdf:resource="&xsd;string"/>
	</owl:AnnotationProperty>
	
	<owl:Class rdf:about="&dtype;CodeList">
		<rdfs:subClassOf rdf:resource="&dtype;Enumeration"/>
		<rdfs:label>Codelist</rdfs:label>
		<dcterms:description>A codelist is a controlled vocabulary of terms that are used to represent permissible values of a 
variable in information systems. 
The representaiton of codes in &quot;dtype&quot; has been influenced by CCTS and UBL.</dcterms:description>
		<rdfs:isDefinedBy rdf:resource="http://www.linkedmodel.org/schema/dtype"/>
	</owl:Class>
	
	<owl:Class rdf:about="&dtype;CompositeCodeList">
		<rdfs:subClassOf rdf:resource="&dtype;CodeList"/>
		<rdfs:subClassOf>
			<owl:Restriction>
				<owl:onProperty rdf:resource="&dtype;compositeOf"/>
				<owl:allValuesFrom rdf:resource="&dtype;CodeList"/>
			</owl:Restriction>
		</rdfs:subClassOf>
		<rdfs:label>Composite Code List</rdfs:label>
		<dcterms:description>A composite codelist is a codelist made up of other codelists. 
It does not introduce any new codes.</dcterms:description>
		<rdfs:isDefinedBy rdf:resource="http://www.linkedmodel.org/schema/dtype"/>
		<owl:disjointWith rdf:resource="&dtype;DerivedCodeList"/>
		<owl:disjointWith rdf:resource="&dtype;SimpleCodeList"/>
	</owl:Class>
	
	<owl:Class rdf:about="&dtype;DerivedCodeList">
		<rdfs:subClassOf rdf:resource="&dtype;CodeList"/>
		<rdfs:subClassOf>
			<owl:Restriction>
				<owl:onProperty rdf:resource="&dtype;derivedFrom"/>
				<owl:allValuesFrom rdf:resource="&dtype;CodeList"/>
			</owl:Restriction>
		</rdfs:subClassOf>
		<rdfs:subClassOf>
			<owl:Restriction>
				<owl:onProperty rdf:resource="&dtype;hasMember"/>
				<owl:allValuesFrom rdf:resource="&dtype;ValueReference"/>
			</owl:Restriction>
		</rdfs:subClassOf>
		<rdfs:subClassOf>
			<owl:Restriction>
				<owl:onProperty rdf:resource="&dtype;derivedFrom"/>
				<owl:maxCardinality rdf:datatype="&xsd;integer">1</owl:maxCardinality>
			</owl:Restriction>
		</rdfs:subClassOf>
		<rdfs:label>Derived Code List</rdfs:label>
		<dcterms:description>A derived codelist is a sublist of another codelist. 
The members that it has must be members of the source list.</dcterms:description>
		<rdfs:isDefinedBy rdf:resource="http://www.linkedmodel.org/schema/dtype"/>
		<owl:disjointWith rdf:resource="&dtype;CompositeCodeList"/>
		<owl:disjointWith rdf:resource="&dtype;SimpleCodeList"/>
	</owl:Class>
	
	<owl:Class rdf:about="&dtype;EnumeratedValue">
		<rdfs:subClassOf rdf:resource="&owl;Thing"/>
		<rdfs:subClassOf>
			<owl:Restriction>
				<owl:onProperty rdf:resource="&dtype;value"/>
				<owl:cardinality rdf:datatype="&xsd;integer">1</owl:cardinality>
			</owl:Restriction>
		</rdfs:subClassOf>
		<rdfs:subClassOf>
			<owl:Restriction>
				<owl:onProperty rdf:resource="&dtype;code"/>
				<owl:maxCardinality rdf:datatype="&xsd;integer">1</owl:maxCardinality>
			</owl:Restriction>
		</rdfs:subClassOf>
		<rdfs:subClassOf>
			<owl:Restriction>
				<owl:onProperty rdf:resource="&dtype;literal"/>
				<owl:maxCardinality rdf:datatype="&xsd;integer">1</owl:maxCardinality>
			</owl:Restriction>
		</rdfs:subClassOf>
		<rdfs:subClassOf>
			<owl:Restriction>
				<owl:onProperty rdf:resource="&dtype;order"/>
				<owl:maxCardinality rdf:datatype="&xsd;integer">1</owl:maxCardinality>
			</owl:Restriction>
		</rdfs:subClassOf>
		<rdfs:label>DTYPE Enumerated Value</rdfs:label>
		<dcterms:description>The base class for datatypes that have values that are restriced to a set of literals or tokens. 
The members of the restriction may themselves be restriced by facets that apply to scalar data types.</dcterms:description>
		<rdfs:isDefinedBy rdf:resource="http://www.linkedmodel.org/schema/dtype"/>
	</owl:Class>
	
	<owl:Class rdf:about="&dtype;Enumeration">
		<rdfs:subClassOf rdf:resource="&owl;Thing"/>
		<rdfs:subClassOf>
			<owl:Restriction>
				<owl:onProperty rdf:resource="&dtype;defaultObjectValue"/>
				<owl:allValuesFrom rdf:resource="&dtype;EnumeratedValue"/>
			</owl:Restriction>
		</rdfs:subClassOf>
		<rdfs:subClassOf>
			<owl:Restriction>
				<owl:onProperty rdf:resource="&dtype;objectValue"/>
				<owl:allValuesFrom rdf:resource="&dtype;EnumeratedValue"/>
			</owl:Restriction>
		</rdfs:subClassOf>
		<rdfs:subClassOf>
			<owl:Restriction>
				<owl:onProperty rdf:resource="&dtype;objectValue"/>
				<owl:allValuesFrom rdf:resource="&dtype;EnumeratedValue"/>
			</owl:Restriction>
		</rdfs:subClassOf>
		<rdfs:subClassOf>
			<owl:Restriction>
				<owl:onProperty rdf:resource="&dtype;defaultObjectValue"/>
				<owl:maxCardinality rdf:datatype="&xsd;integer">1</owl:maxCardinality>
			</owl:Restriction>
		</rdfs:subClassOf>
		<rdfs:subClassOf>
			<owl:Restriction>
				<owl:onProperty rdf:resource="&dtype;objectValue"/>
				<owl:minCardinality rdf:datatype="&xsd;integer">1</owl:minCardinality>
			</owl:Restriction>
		</rdfs:subClassOf>
		<rdfs:label>DTYPE Enumeration</rdfs:label>
		<dcterms:description>A type that serves as a container for the enumerated values of an enumeration. 
This enables the enumeration itself to be referenceable. 
One need for this is in determing the default value of an enumeration.
Another need is in the management of sub-enumerations and composite enumerations.</dcterms:description>
		<rdfs:isDefinedBy rdf:resource="http://www.linkedmodel.org/schema/dtype"/>
	</owl:Class>
	
	<vaem:GraphMetaData rdf:about="&dtype;GMD_DTYPE">
		<rdfs:label>DTYPE Schema Version 2.1 Metadata</rdfs:label>
		<dcterms:created rdf:datatype="&xsd;date">2011-05-29</dcterms:created>
		<dcterms:modified rdf:datatype="&xsd;date">2023-11-14</dcterms:modified>
		<dcterms:title>DTYPE Version 2.1 Metadata</dcterms:title>
		<vaem:description>The ontology &quot;dtype&quot; provides a specification of simple data types such as enumerations and codelists. 
These are needed in support of the conversion of XML Schemas and UML Models to OWL. 
The purpose of &quot;dtype&quot; is to provide a foundation for expressing rich data types. 
These data types are typically needed when dealing with OWL representations of data structures derived from XML Schema.</vaem:description>
		<vaem:hasGraphRole rdf:resource="&vaem;SchemaGraph"/>
		<vaem:hasLicenseType rdf:resource="http://voag.linkedmodel.org/voag/CC-SHAREALIKE_3PT0-US"/>
		<vaem:hasOwner rdf:resource="&vaem;TopQuadrant"/>
		<vaem:hasSteward rdf:resource="&vaem;TopQuadrant"/>
		<vaem:intent>The purpose of DTYPE is to provide, by import, a foundation for  data types.</vaem:intent>
		<vaem:latestPublishedVersion rdf:datatype="&xsd;anyURI">http://www.linkedmodel.org/doc/2023/SCHEMA_dtype</vaem:latestPublishedVersion>
		<vaem:logo rdf:datatype="&xsd;anyURI">http://www.linkedmodel.org/lib/lm/images/logos/dtype_logo-300x110.png</vaem:logo>
		<vaem:name>DTYPE</vaem:name>
		<vaem:namespace rdf:datatype="&xsd;anyURI">http://www.linkedmodel.org/schema/dtype#</vaem:namespace>
		<vaem:namespacePrefix>dtype</vaem:namespacePrefix>
		<vaem:owner>LinkedModel.org</vaem:owner>
		<vaem:previousPublishedVersion rdf:datatype="&xsd;anyURI">http://www.linkedmodel.org/doc/2015/SCHEMA_dtype-v1.2</vaem:previousPublishedVersion>
		<vaem:releaseDate rdf:datatype="&xsd;date">2023-11-14</vaem:releaseDate>
		<vaem:revision>2.1</vaem:revision>
		<vaem:title>Datatype Schema (DTYPE) - Version 2.1</vaem:title>
		<vaem:turtleFileURL rdf:datatype="&xsd;anyURI">http://www.linkedmodel.org/dtype/schema/SCHEMA_dtype.ttl</vaem:turtleFileURL>
		<vaem:usesNonImportedResource rdf:resource="&dcterms;abstract"/>
		<vaem:usesNonImportedResource rdf:resource="&dcterms;author"/>
		<vaem:usesNonImportedResource rdf:resource="&dcterms;created"/>
		<vaem:usesNonImportedResource rdf:resource="&dcterms;modified"/>
		<vaem:usesNonImportedResource rdf:resource="&dcterms;title"/>
		<vaem:usesNonImportedResource rdf:resource="http://voag.linkedmodel.org/voag/CC-SHAREALIKE_3PT0-US"/>
		<vaem:withAttributionTo>DTYPE is issued under a Creative Commons Attribution Share Alike 3.0 United States License.</vaem:withAttributionTo>
		<rdfs:isDefinedBy rdf:resource="http://www.linkedmodel.org/schema/dtype"/>
	</vaem:GraphMetaData>
	
	<owl:Class rdf:about="&dtype;SimpleCodeList">
		<rdfs:subClassOf rdf:resource="&dtype;CodeList"/>
		<rdfs:subClassOf>
			<owl:Restriction>
				<owl:onProperty rdf:resource="&dtype;hasMember"/>
				<owl:allValuesFrom rdf:resource="&dtype;EnumeratedValue"/>
			</owl:Restriction>
		</rdfs:subClassOf>
		<rdfs:label>Simple Code List</rdfs:label>
		<dcterms:description>A simple codelist is one made up only of enumerated values.</dcterms:description>
		<rdfs:isDefinedBy rdf:resource="http://www.linkedmodel.org/schema/dtype"/>
		<owl:disjointWith rdf:resource="&dtype;CompositeCodeList"/>
		<owl:disjointWith rdf:resource="&dtype;DerivedCodeList"/>
	</owl:Class>
	
	<owl:Class rdf:about="&dtype;ValueReference">
		<rdfs:subClassOf rdf:resource="&owl;Thing"/>
		<rdfs:subClassOf>
			<owl:Restriction>
				<owl:onProperty rdf:resource="&dtype;refersTo"/>
				<owl:allValuesFrom rdf:resource="&dtype;EnumeratedValue"/>
			</owl:Restriction>
		</rdfs:subClassOf>
		<rdfs:subClassOf>
			<owl:Restriction>
				<owl:onProperty rdf:resource="&dtype;refersTo"/>
				<owl:cardinality rdf:datatype="&xsd;integer">1</owl:cardinality>
			</owl:Restriction>
		</rdfs:subClassOf>
		<rdfs:subClassOf>
			<owl:Restriction>
				<owl:onProperty rdf:resource="&dtype;order"/>
				<owl:maxCardinality rdf:datatype="&xsd;integer">1</owl:maxCardinality>
			</owl:Restriction>
		</rdfs:subClassOf>
		<rdfs:label>Value Reference</rdfs:label>
		<dcterms:description>A value reference is a pointer to an Enumerated Value. 
The original order of the value can be overridden by the &quot;order&quot; attribute.</dcterms:description>
		<rdfs:isDefinedBy rdf:resource="http://www.linkedmodel.org/schema/dtype"/>
	</owl:Class>
	
	<owl:DatatypeProperty rdf:about="&dtype;code">
		<rdfs:label>code</rdfs:label>
		<rdfs:comment>A unique value that is assigned to an enumeration member.</rdfs:comment>
		<dcterms:description>A property for expressing a unique value for a member of an enumeration. 
The range has been set to &quot;xsd:anySimpleType&quot; to allow for any scalar datatype.</dcterms:description>
		<rdfs:isDefinedBy rdf:resource="http://www.linkedmodel.org/schema/dtype"/>
		<rdfs:range rdf:resource="&xsd;anySimpleType"/>
	</owl:DatatypeProperty>
	
	<owl:ObjectProperty rdf:about="&dtype;compositeOf">
		<rdfs:label>composite of</rdfs:label>
		<dcterms:description>A property for constructing composite data structures</dcterms:description>
		<rdfs:isDefinedBy rdf:resource="http://www.linkedmodel.org/schema/dtype"/>
	</owl:ObjectProperty>
	
	<rdfs:Datatype rdf:about="&dtype;dateUnion">
		<rdfs:subClassOf rdf:resource="&rdfs;Resource"/>
		<rdfs:label>date union</rdfs:label>
		<dcterms:description>A datatype that is the union of date datatypes.</dcterms:description>
		<rdfs:isDefinedBy rdf:resource="http://www.linkedmodel.org/schema/dtype"/>
		<owl:equivalentClass>
			<owl:Class>
				<owl:unionOf rdf:parseType="Collection">
					<rdf:Description rdf:about="&xsd;date">
					</rdf:Description>
					<rdf:Description rdf:about="&xsd;dateTime">
					</rdf:Description>
					<rdf:Description rdf:about="&xsd;gYear">
					</rdf:Description>
					<rdf:Description rdf:about="&xsd;gMonth">
					</rdf:Description>
					<rdf:Description rdf:about="&xsd;gMonthDay">
					</rdf:Description>
					<rdf:Description rdf:about="&xsd;gYearMonth">
					</rdf:Description>
					<rdf:Description rdf:about="&xsd;gDay">
					</rdf:Description>
				</owl:unionOf>
			</owl:Class>
		</owl:equivalentClass>
	</rdfs:Datatype>
	
	<owl:ObjectProperty rdf:about="&dtype;defaultObjectValue">
		<rdfs:label>default object value</rdfs:label>
		<dcterms:description>The property &quot;dtype:defaultValue&quot; is a general property for specifying an object value in situations where 
none is specified.</dcterms:description>
		<rdfs:isDefinedBy rdf:resource="http://www.linkedmodel.org/schema/dtype"/>
	</owl:ObjectProperty>
	
	<owl:DatatypeProperty rdf:about="&dtype;defaultValue">
		<rdfs:label>default value</rdfs:label>
		<dcterms:description>The property &quot;dtype:defaultValue&quot; is a general property for specifying a literal value in situations where 
none is specified.</dcterms:description>
		<rdfs:isDefinedBy rdf:resource="http://www.linkedmodel.org/schema/dtype"/>
	</owl:DatatypeProperty>
	
	<owl:ObjectProperty rdf:about="&dtype;derivedFrom">
		<rdfs:label>derived from</rdfs:label>
		<dcterms:description>A property for specifying a derivation relationship.</dcterms:description>
		<rdfs:isDefinedBy rdf:resource="http://www.linkedmodel.org/schema/dtype"/>
	</owl:ObjectProperty>
	
	<owl:ObjectProperty rdf:about="&dtype;hasMember">
		<rdfs:label>has member</rdfs:label>
		<dcterms:description>A property for specifying how member elements make up a data structure.</dcterms:description>
		<rdfs:isDefinedBy rdf:resource="http://www.linkedmodel.org/schema/dtype"/>
	</owl:ObjectProperty>
	
	<owl:DatatypeProperty rdf:about="&dtype;isInvalid">
		<rdfs:label>is invalid</rdfs:label>
		<dcterms:description>A boolean flag to state that a value is invalid with respect to its type.</dcterms:description>
		<rdfs:isDefinedBy rdf:resource="http://www.linkedmodel.org/schema/dtype"/>
		<rdfs:range rdf:resource="&xsd;boolean"/>
	</owl:DatatypeProperty>
	
	<owl:DatatypeProperty rdf:about="&dtype;literal">
		<rdfs:label>literal</rdfs:label>
		<rdfs:comment></rdfs:comment>
		<dcterms:description>A general purpose property for holding string literals as a machine-readable string for how the 
enumerated value can be referred to. 
This can be used when the code value is numeric, as an alternative to using a code. 
Literal is not the same as label which is intended for human readable display. 
For example, a code for January may be 1, the literal may be &apos;J&apos; or &apos;jan&apos; and the label &apos;January&apos;.</dcterms:description>
		<rdfs:isDefinedBy rdf:resource="http://www.linkedmodel.org/schema/dtype"/>
		<rdfs:range rdf:resource="&xsd;string"/>
	</owl:DatatypeProperty>
	
	<rdfs:Datatype rdf:about="&dtype;numericUnion">
		<rdfs:subClassOf rdf:resource="&rdfs;Resource"/>
		<rdfs:label>numeric union</rdfs:label>
		<dcterms:description>A datatype that is the union of numeric xsd data types.
&quot;dtype:numericUnion&quot; is equivalent to the xsd specification that uses an xsd:union of 
memberTypes=&quot;xsd:decimal xsd:double xsd:float xsd:integer&quot;.</dcterms:description>
		<rdfs:isDefinedBy rdf:resource="http://www.linkedmodel.org/schema/dtype"/>
		<owl:equivalentClass>
			<rdfs:Datatype>
				<owl:unionOf rdf:parseType="Collection">
					<rdf:Description rdf:about="&xsd;float">
					</rdf:Description>
					<rdf:Description rdf:about="&xsd;decimal">
					</rdf:Description>
					<rdf:Description rdf:about="&xsd;integer">
					</rdf:Description>
					<rdf:Description rdf:about="&xsd;double">
					</rdf:Description>
				</owl:unionOf>
			</rdfs:Datatype>
		</owl:equivalentClass>
	</rdfs:Datatype>
	
	<owl:ObjectProperty rdf:about="&dtype;objectValue">
		<rdfs:label>object value</rdfs:label>
		<dcterms:description>The property &quot;dtype:objectValue&quot; is a general property for specifying an object value in situations where 
none is specified.</dcterms:description>
		<rdfs:isDefinedBy rdf:resource="http://www.linkedmodel.org/schema/dtype"/>
	</owl:ObjectProperty>
	
	<owl:DatatypeProperty rdf:about="&dtype;order">
		<rdfs:label>order</rdfs:label>
		<dcterms:description>The property &quot;dtype:order&quot; provides a means to specify a precedence. 
One use of order is in specifying ordered enumerations such as &quot;voag:ConfidentialityLevel&quot;.
A similar property, but with an important type difference, is &quot;vaem:orderIndex&quot;.
This is for use on property occurrences in class axioms where it can be placed on a restriction 
to specify how that property may be transformed into other representations where ordering has some 
importance, for example, in XML Schema sequences. 
Whereas &quot;vaem:order&quot; is a datatype property, &quot;vaem:orderIndex&quot; is an annotation property.
The &quot;order&quot; property specifies a value that can establish precedence and ordinality. 
One use of order is in make an enumeration an ordinal type. 
For example &quot;RiskLevel&quot; might have the values &quot;very low&quot;, &quot;low&quot;, &quot;medium&quot;, &quot;high&quot; and &quot;very high&quot;.
A query that asks for all risks that are greater than &quot;medium&quot; would use the ordinal values and return 
those resources that have “medium”, “high” and “very high” ordinality.</dcterms:description>
		<rdfs:isDefinedBy rdf:resource="http://www.linkedmodel.org/schema/dtype"/>
		<rdfs:range rdf:resource="&xsd;integer"/>
		<rdfs:seeAlso rdf:resource="&dtype;orderIndex"/>
	</owl:DatatypeProperty>
	
	<owl:AnnotationProperty rdf:about="&dtype;orderIndex">
		<rdfs:label>order index</rdfs:label>
		<dcterms:description>The property &quot;dtype:orderIndex&quot; is an annotation property to specify a position that some value or 
structure will have. 
One use is to specify the place that a resource has in a sequence.
Another use is on property occurrences in class axioms, where &quot;vaem:orderIndex&quot; is placed on a 
restriction to specify how that property may be transformed into a representation where ordering has 
some importance, for example, in XML Schema sequences.</dcterms:description>
		<rdfs:isDefinedBy rdf:resource="http://www.linkedmodel.org/schema/dtype"/>
		<rdfs:range rdf:resource="&xsd;integer"/>
	</owl:AnnotationProperty>
	
	<owl:ObjectProperty rdf:about="&dtype;refersTo">
		<rdfs:label>refers to</rdfs:label>
		<dcterms:description>An indirection pointer for relating a slot in am occurrence data structure, such as &quot;dtype:ValueReference&quot; with another resource.</dcterms:description>
		<rdfs:isDefinedBy rdf:resource="http://www.linkedmodel.org/schema/dtype"/>
	</owl:ObjectProperty>
	
	<owl:ObjectProperty rdf:about="&dtype;type">
		<rdfs:label>datatype</rdfs:label>
		<rdfs:isDefinedBy rdf:resource="http://www.linkedmodel.org/schema/dtype"/>
	</owl:ObjectProperty>
	
	<owl:DatatypeProperty rdf:about="&dtype;value">
		<rdfs:label>value</rdfs:label>
		<dcterms:description>The property &quot;dtype:value&quot; is a general property for specifying a literal value in situations where 
none is specified.</dcterms:description>
		<rdfs:isDefinedBy rdf:resource="http://www.linkedmodel.org/schema/dtype"/>
		<rdfs:range rdf:resource="&xsd;anySimpleType"/>
	</owl:DatatypeProperty>

</rdf:RDF>